Add rule definitions

TypeSugar2.v
@@ -1,7 +1,7 @@
 Require Export SystemFR.ShiftOpen.
 
-Definition tsingleton t :=
-  T_type_refine T_top (T_equiv (lvar 0 term_var) (shift 0 t 1)).
+Definition tsingleton T t :=
+  T_type_refine T (T_equiv (lvar 0 term_var) (shift 0 t 1)).
 
 Definition type_application T1 T2 : tree :=
   T_type_refine T_top (
@@ -18,32 +18,24 @@ Definition List : tree :=
     (T_sum T_unit (T_prod T_top (lvar 0 type_var))).
 
 Definition tnil := tleft uu.
-Definition Nil := tsingleton tnil.
+Definition Nil := tsingleton List tnil.
 
 Definition Var x := tsingleton (fvar x term_var).
 
 Definition tcons h t := tright (pp h t).
 Definition Cons H T :=
   T_exists H (T_exists T (
-    tsingleton (tcons (lvar 1 term_var) (lvar 0 term_var))
+    tsingleton List (tcons (lvar 1 term_var) (lvar 0 term_var))
   )).
 
-Definition Match T1 T2 T3 :=
-  T_exists T1 (
-    T_union
-      (T_type_refine T2 (T_equiv (lvar 1 term_var) (tleft uu)))
-      (T_exists T_top (
-        (T_exists List (
-          (T_type_refine
-            (shift 0 T3 1)
-            (T_equiv
-               (lvar 3 term_var)
-               (tright (pp (lvar 2 term_var) (lvar 1 term_var))))
-          )
-        ))
+Definition List_Match t T2 T3 :=
+  T_union
+    (T_type_refine T2 (T_equiv t tnil))
+    (T_exists T_top (
+      (T_exists List (
+        (T_type_refine T3 (T_equiv t (tcons (lvar 2 term_var) (lvar 1 term_var))))
       ))
-  ).
-
+    )).
 
 (*
 default: T
@@ -61,9 +53,9 @@ val f = f'(globalFuel)
 
 Parameter globalFuel: tree.
 
-Definition fix_default t default : tree :=
+Definition fix_default t default fuel: tree :=
   app
-    (notype_lambda (app (lvar 0 term_var) globalFuel))
+    (notype_lambda (app (lvar 0 term_var) fuel))
     (notype_tfix (
       notype_lambda (              (* fuel *)
         tmatch (lvar 0 term_var)   (* fuel *)
@@ -76,11 +68,12 @@ Definition fix_default t default : tree :=
     ).
 
 Lemma wf_fix_default:
-  forall default t,
+  forall default t fuel,
     wf globalFuel 0 ->
     wf t 1 ->
     wf default 0 ->
-    wf (fix_default t default) 0.
+    wf fuel 0 ->
+    wf (fix_default t default fuel) 0.
 Proof.
   unfold fix_default;
     repeat step;
